src/PlutusIR/Transform/LetNonRec/DecideBool.v
@@ -2,96 +2,113 @@ From Coq Require Import
   String
   List
   Bool
-  Program.
+  Program
+  Datatypes
+  Utf8_core
+  PeanoNat
+.
 
 From PlutusCert Require Import
   Util
+  Util.Tactics
+  Util.List
   PlutusIR
   PlutusIR.Analysis.Equality
   PlutusIR.Transform.Compat
   PlutusIR.Transform.LetNonRec.Spec.
 Import NamedTerm.
 
+Import ListNotations.
+
 (*
    Returns `Just t'` if bindings were desugared correctly, where t' is the rest
    of the desugared term.
 
-   Note that Term_desugar has to be passed manually. In this form, the
-   termination checker is happy when checking Term_desugar (it's probably
-   inlining Bindings_desugar within Term_desugar, and then sees the structural
-   recursive call to Term_desugar.
+   Note that dec_Term has to be passed manually. In this form, the
+   termination checker is happy when checking dec_Term (it's probably
+   inlining dec_Bindings within dec_Term, and then sees the structural
+   recursive call to dec_Term.
 
    We want this as a separate definition so that proofs don't have to deal with
    a big (fix ...) expression. The termination checker doesn't allow it to be
-   part of the mutual recursive binding group of Term_desugar, so this is the
+   part of the mutual recursive binding group of dec_Term, so this is the
    workaround.
 
-   Below is a specialized version Bindings_desugar that you do not have to pass
-   Term_desugar.
+   Below is a specialized version dec_Bindings that you do not have to pass
+   dec_Term.
 *)
-Definition Bindings_desugar' :=
-  fun (Term_desugar : Term -> Term -> bool) =>
-    (fix Bindings_desugar'
-            (bs : list Binding) (t : Term) {struct bs} := match bs with
-            | nil       => Just t
-            | cons b bs => match b, t with
-              | TermBind Strict (VarDecl v ty) rhs, Apply (LamAbs v' ty' body') rhs' =>
-                if (String.eqb v v' && Ty_eqb ty ty' && Term_desugar rhs rhs')
-                  then Bindings_desugar' bs body'
-                  else None
-                (* Notation scope analysis fails, not sure why....*)
-              | _, _ => None
-              end
-            end).
+
+Section Bindings.
+
+  Context (dec_Term : Term -> Term -> bool).
+
+  Fixpoint bindings_to_apps (bs : list Binding) : option (list (Term -> Term)) :=
+    match bs with
+      | []        => Just []
+      | TermBind Strict (VarDecl v ty) rhs :: bs =>
+          option_map
+            (cons (fun t => Apply (LamAbs v ty t) rhs))
+            (bindings_to_apps bs)
+      |  _ => None
+    end.
+
+  Fixpoint dec_Bindings' (bs : list Binding) (t : Term) {struct bs} : option Term :=
+    match bs with
+      | nil       => Just t
+      | cons b bs => match b, t with
+        | TermBind Strict (VarDecl v ty) rhs, Apply (LamAbs v' ty' body') rhs' =>
+          if (String.eqb v v' && Ty_eqb ty ty' && dec_Term rhs rhs')
+            then dec_Bindings' bs body'
+            else None
+        | _, _ => None
+        end
+    end.
+
+End Bindings.
 
 (*
   Returns true if the term was desugared correctly.
 *)
-Fixpoint Term_desugar (x y : Term) {struct x} : bool := match x, y with
-
-  (* We don't allow empty binding groups. This should be visible
-     from the AST type (as it is in plutus implementation)
-  *)
-  | Let _ nil _ , _ => false
+Fixpoint dec_Term (x y : Term) {struct x} : bool := match x, y with
 
   (* non-recursive bindings should be desugared *)
   | Let NonRec bs body, t =>
-       match Bindings_desugar' Term_desugar bs t with
-        | Just body' => Term_desugar body body'
+       match dec_Bindings' dec_Term bs t with
+        | Just body' => dec_Term body body'
         | Nothing    => false
        end
 
   (* Other cases should be compatible, i.e. identical constructors
      and recursive Terms recursively desugared *)
-  | Let Rec bs t, Let Rec bs' t' =>
-      list_eqb Binding_desugar bs bs'
-        && Term_desugar t t'
+  | Let Rec bs t   , Let Rec bs' t'     => forall2b dec_Binding_compat bs bs' && dec_Term t t'
   | Var n          , Var n'             => String.eqb n n'
-  | TyAbs n k t    , TyAbs n' k' t'     => String.eqb n n' && Kind_eqb k k' && Term_desugar t t'
-  | LamAbs n ty t  , LamAbs n' ty' t'   => String.eqb n n' && Ty_eqb ty ty' && Term_desugar t t'
-  | Apply s t      , Apply s' t'        => Term_desugar s s' && Term_desugar t t'
+  | TyAbs n k t    , TyAbs n' k' t'     => String.eqb n n' && Kind_eqb k k' && dec_Term t t'
+  | LamAbs n ty t  , LamAbs n' ty' t'   => String.eqb n n' && Ty_eqb ty ty' && dec_Term t t'
+  | Apply s t      , Apply s' t'        => dec_Term s s' && dec_Term t t'
   | Constant c     , Constant c'        => some_valueOf_eqb c c'
   | Builtin f      , Builtin f'         => func_eqb f f'
-  | TyInst t ty    , TyInst t' ty'      => Term_desugar t t' && Ty_eqb ty ty'
+  | TyInst t ty    , TyInst t' ty'      => dec_Term t t' && Ty_eqb ty ty'
   | Error ty       , Error ty'          => Ty_eqb ty ty'
-  | IWrap ty1 ty2 t, IWrap ty1' ty2' t' => Ty_eqb ty1 ty1' && Ty_eqb ty2 ty2' && Term_desugar t t'
-  | Unwrap t       , Unwrap t'          => Term_desugar t t'
+  | IWrap ty1 ty2 t, IWrap ty1' ty2' t' => Ty_eqb ty1 ty1' && Ty_eqb ty2 ty2' && dec_Term t t'
+  | Unwrap t       , Unwrap t'          => dec_Term t t'
+  | Constr i ts    , Constr i' ts'      => Nat.eqb i i' && list_eqb dec_Term ts ts'
+  | Case t ts      , Case t' ts'        => dec_Term t t' && list_eqb dec_Term ts ts'
 
   | _, _ => false
   end
-with Binding_desugar (b b' : Binding) : bool := match b, b' with
+with dec_Binding_compat (b b' : Binding) : bool := match b, b' with
   (* These cases are only used for recursive let-bindings, i.e.
      equal and recursive Terms should be desugared *)
-  | TermBind s vdecl t, TermBind s' vdecl' t' => Strictness_eqb s s' && VDecl_eqb vdecl vdecl' && Term_desugar t t'
+  | TermBind s vdecl t, TermBind s' vdecl' t' => Strictness_eqb s s' && VDecl_eqb vdecl vdecl' && dec_Term t t'
   | TypeBind tvdecl ty, TypeBind tvdecl' ty'  => TVDecl_eqb tvdecl tvdecl' && Ty_eqb ty ty'
   | DatatypeBind dtd  , DatatypeBind dtd'     => DTDecl_eqb dtd dtd'
   | _, _ => false
   end
 .
 
-(* See comment of Bindings_desugar' *)
-Definition Bindings_desugar
-     : list Binding -> Term -> option Term := Bindings_desugar' Term_desugar.
+(* See comment of dec_Bindings' *)
+Definition dec_Bindings : list Binding -> Term -> option Term := 
+  dec_Bindings' dec_Term.
 
 
 (*
@@ -101,7 +118,7 @@ Note [IH for nested datatypes]
 Usual IH used by `induction` tactic does not suffice, it only holds
 for _direct_ subterms, and not for subterms within a list subterm.
 
-- Define an induction/recursion scheme similarly to Term_desugar above.
+- Define an induction/recursion scheme similarly to dec_Term above.
 *)
 
 
@@ -120,13 +137,258 @@ or argument.
 
 *)
 
+Definition P_Term t := ∀ t',
+  dec_Term t t' = true <-> CNR_Term t t'.
+
+Definition P_Binding_compat b :=  ∀ b',
+    dec_Binding_compat b b' = true <-> CNR_Binding_compat b b'
+.
+
+Definition P_Binding_NonRec b := ∀ t t_inner,
+  (∃ bs, dec_Bindings (b :: bs) t = Some t_inner) <->
+  (∃ f fs,
+    CNR_Binding b f /\
+    fold_right apply t_inner (f :: fs) = t)
+.
+
+Definition P_Binding b :=
+  P_Binding_compat b /\ P_Binding_NonRec b
+.
+
+Ltac simpl_dec_Term :=
+  try match goal with (* Try because not used in Binding cases *)
+    | H:dec_Term _ _ = true |- _ => simpl in H
+  end;
+  repeat (match goal with
+    | H : match ?r with _ => _ end = true |- _ => destruct r
+    | H : false = true |- _ => inversion H
+    | H : _ && _ = true |- _ => rewrite andb_true_iff in H
+    | H : _ /\ _ |- _ => destruct H in H
+  end).
+
+Ltac rewrite_reflection :=
+  repeat (match goal with
+
+    | H : String.eqb _ _ = true |- _ => rewrite String.eqb_eq in H
+    | H : Kind_eqb _ _ = true |- _ => rewrite Kind_eqb_eq in H
+    | H : Ty_eqb _ _ = true |- _ => rewrite Ty_eqb_eq in H
+    | H : some_valueOf_eqb _ _ = true |- _ => rewrite some_valueOf_eqb_eq in H
+    | H : func_eqb _ _ = true |- _ => rewrite func_eqb_eq in H
+    | H : Nat.eqb _ _ = true |- _ => rewrite Nat.eqb_eq in H
+    | H : Strictness_eqb _ _ = true |- _ => rewrite Strictness_eqb_eq in H
+    | H : VDecl_eqb _ _ = true |- _ => rewrite VDecl_eqb_eq in H
+    | H : list_eqb ?eqb ?xs _ = true,
+      H_elems : ForallP _ ?xs |- _
+        => rewrite ForallP_Forall in H_elems;
+           rewrite (forall2b_Forall2_Forall _ _ dec_Term xs _ H_elems) in H
+
+    | H : dec_Term ?t ?t' = true ,
+      IH : _ -> dec_Term ?t _ = true <-> _ |- _ => rewrite IH in H
+  end).
+
+
+Ltac tac_fwd :=
+  intros;
+  simpl_dec_Term;
+  rewrite_reflection;
+  subst;
+  auto using CNR_Term.
+
+
+Ltac simpl_goal :=
+  simpl;
+  repeat (rewrite andb_true_iff)
+.
+
+Ltac bwd_reflection :=
+  repeat (match goal with
+    | |- String.eqb _ _ = true => rewrite String.eqb_eq; reflexivity
+    | |- Kind_eqb _ _ = true   => rewrite Kind_eqb_eq; reflexivity
+    | |- Ty_eqb _ _ = true   => rewrite Ty_eqb_eq; reflexivity
+    | |- some_valueOf_eqb _ _ = true => rewrite some_valueOf_eqb_eq; reflexivity
+    | |- func_eqb _ _ = true => rewrite func_eqb_eq; reflexivity
+    | |- Nat.eqb _ _ = true => rewrite Nat.eqb_eq; reflexivity
+    | |- Strictness_eqb _ _ = true => rewrite Strictness_eqb_eq; reflexivity
+    | |- VDecl_eqb _ _ = true => rewrite VDecl_eqb_eq; reflexivity
+
+    |
+      H_elems : ForallP _ ?xs |- list_eqb ?eqb ?xs _ = true =>
+        rewrite ForallP_Forall in H_elems;
+        rewrite (forall2b_Forall2_Forall _ CNR_Term dec_Term xs _ H_elems);
+        assumption
+    | IH : _ -> dec_Term ?t _ = true <-> _ |- dec_Term ?t _ = true => rewrite IH; assumption
+  end).
+
+Ltac tac_bwd :=
+  inversion 1; subst;
+  simpl_goal;
+  repeat split;
+  bwd_reflection.
+
+Ltac dec_tac :=
+  unfold P_Term, P_Binding;
+  intros;
+
+  (* Split cases, solve impossible ones *)
+  match goal with t' : Term |- _ =>
+    destruct t'; split; try solve [inversion 1]
+  end; [> tac_fwd | tac_bwd].
+
+Definition desugar_fun v ty t_bound : Term -> Term :=
+  fun t_inner => Apply (LamAbs v ty t_inner) t_bound.
+
+Lemma dec_Bindings_exists : ∀ bs t t_inner,
+  dec_Bindings bs t = Some t_inner ->
+  (∃ fs, fold_right apply t_inner fs = t)
+.
+Proof.
+  induction bs as [ | b bs].
+  - simpl. intros. inversion H. subst t_inner.
+    exists []. auto.
+  - intros.
+    destruct b;
+    try solve [inversion H].
+    destruct s; try solve [inversion H].
+    destruct v.
+    simpl in H.
+    destruct t; try solve [inversion H].
+    destruct t2; try solve [inversion H].
+    destruct ((s =? s0)%string && Ty_eqb t1 t && dec_Term t0 t3); try solve [inversion H].
+    specialize (IHbs _ _ H).
+
+    destruct IHbs as [fs H_fs].
+
+    exists (
+      desugar_fun s0 t t3
+      ::
+      fs).
+    unfold desugar_fun.
+    subst t2.
+    simpl.
+    reflexivity.
+Qed.
+
+Lemma dec_funs_exists : ∀ fs t t_inner,
+  Forall (fun f => ∃ v ty t_bound, f = desugar_fun v ty t_bound) fs ->
+  fold_right apply t_inner fs = t ->
+  ∃ bs, dec_Bindings bs t = Some t_inner
+.
+Proof.
+  admit.
+Admitted.
+
+Definition dec_Term_equiv : ∀ t, P_Term t.
+Proof.
+  apply Term__multind with (P := P_Term) (Q := P_Binding).
+  all: try solve [dec_tac].
+  - (* P_Term Let *)
+    destruct rec.
+    + (* NonRec *)
+      admit.
+    + (* Rec *)
+      unfold P_Term, P_Binding;
+      intros;
+
+      (* Split cases, solve impossible ones *)
+      match goal with t' : Term |- _ =>
+        destruct t'; split; try solve [inversion 1]
+      end.
+      * (*fwd *) 
+      intros.
+      simpl_dec_Term.
+      rewrite ForallP_Forall in *.
+      apply (Forall_impl P_Binding_compat (fun b H => proj1 H)) in H.
+        unfold P_Binding_compat in *.
+      apply (forall2b_Forall2_Forall _ _ dec_Binding_compat _ _ H) in H1.
+
+      apply H0 in H2.
+      constructor; auto.
+      generalize dependent l.
+      induction bs.
+      -- intros l H1. inversion H1. constructor.
+      -- intros l H1. inversion H1; subst.
+         apply Forall_inv_tail in H.
+         constructor; eauto.
+      (* bwd *)
+      * intros H_Let.
+        inversion H_Let. subst.
+        simpl.
+        rewrite andb_true_iff.
+        split.
+        -- rewrite ForallP_Forall in H.
+        apply (Forall_impl P_Binding_compat (fun b H => proj1 H)) in H.
+        apply (forall2b_Forall2_Forall _ _ dec_Binding_compat _ _ H).
+        generalize dependent l.
+        induction bs.
+        --- intros l H_Let H_compat.
+            inversion H_compat. subst. constructor.
+        --- intros l H_Let H_compat. inversion H_compat; subst.
+            constructor; auto.
+            inversion H_Let; subst.
+            inversion H9; subst.
+            eapply IHbs; eauto using Forall_inv_tail.
+            eauto using CNR_Term.
+        -- rewrite H0. assumption.
+  - (* P_Binding TermBind *)
+  unfold P_Term, P_Binding;
+  unfold P_Binding_compat, P_Binding_NonRec.
+  intros.
+  split.
+  + (* compat *)
+    split.
+    * (* fwd*)
+      destruct b'; try solve [inversion 1].
+      intros.
+      simpl in H0.
+      simpl_dec_Term.
+      rewrite_reflection.
+      subst.
+      eauto using CNR_Binding_compat.
+    * (* bwd *)
+      destruct b'; try solve [inversion 1].
+      inversion 1; subst.
+      simpl_goal.
+      repeat split; bwd_reflection.
+  + (* P_Binding_NonRec *)
+    intros.
+    split.
+    * (* ∃ fs *)
+      intros.
+      destruct H0.
+      (* simplify dec_Bindings *)
+      destruct s;
+        try solve [inversion H0]. (* Impossible case*)
+      destruct v.
+      simpl in H0.
+      repeat (match goal with
+        | H : match ?t with _ => _ end = _ |- _ => destruct t
+      end); try solve [inversion H0].
+
+      exists (desugar_fun s0 t0 t0_2).
+      apply dec_Bindings_exists in H0 as [fs H_fs].
+      exists fs.
+      split.
+      ** admit.
+      ** unfold apply, desugar_fun. subst t0_1. simpl. reflexivity.
+    * admit.
+
+  - (* P_Binding TypeBind *)
+    intros.
+    unfold P_Binding, P_Binding_compat, P_Binding_NonRec.
+    split; admit.
+  - (* P_Binding DatatypeBind *)
+    admit.
+Admitted.
+
+
+
 Definition Binding_soundness (b : Binding) :=
-  forall s v t, b = TermBind s v t -> forall t' (H_dec_true : Term_desugar t t' = true), CNR_Term t t'.
+  forall s v t, b = TermBind s v t -> forall t' (H_dec_true : dec_Term t t' = true), CNR_Term t t'.
 
 Definition Term_soundness (t : Term) :=
-  forall t', forall (H_dec_true : Term_desugar t t' = true), CNR_Term t t'.
+  forall t', forall (H_dec_true : dec_Term t t' = true), CNR_Term t t'.
 
-(* Prove that Bindings_desugar' is sound w.r.t CNR_Bindings *)
+(* Prove that dec_Bindings' is sound w.r.t CNR_Bindings *)
 Lemma sound_dec_bindings {bs t_let_body' t_result}
   (* Every bound term has sound desugaring *)
   ( IH_bindings : ForallT
@@ -136,7 +398,7 @@ Lemma sound_dec_bindings {bs t_let_body' t_result}
       bs
   )
 
-  ( dec_true : Bindings_desugar' Term_desugar bs t_result = Just t_let_body' )
+  ( dec_true : dec_Bindings' dec_Term bs t_result = Just t_let_body' )
   : {bs_fs & CNR_Bindings bs bs_fs
            & fold_right apply t_let_body' bs_fs = t_result}.
 Proof. Admitted.
@@ -166,7 +428,7 @@ Proof. Admitted.
           rename X0 into sound_bs.
           clear IH_bindings.
 
-          (* destruct until we hit the right branch of Bindings_desugar' in dec_b_bs_true *)
+          (* destruct until we hit the right branch of dec_Bindings' in dec_b_bs_true *)
           destruct t_result.
           all: try inversion dec_b_bs_true.
           destruct t_result1 eqn:H_t_result1.
@@ -178,7 +440,7 @@ Proof. Admitted.
 
           (* reflection *)
           simpl in dec_b_bs_true.
-          destruct ((v =? s)%string && Term_desugar t_bound t_bound') as []eqn:H_v_eq_t_eq.
+          destruct ((v =? s)%string && dec_Term t_bound t_bound') as []eqn:H_v_eq_t_eq.
             (* = false*)
             2: { inversion dec_b_bs_true. }
           bool_assumptions.
@@ -223,7 +485,7 @@ Defined.*)
 
 
 
-Definition Term_desugar_sound t t' : Term_desugar t t' = true -> CNR_Term t t'.
+Definition dec_Term_sound t t' : dec_Term t t' = true -> CNR_Term t t'.
 Proof. Admitted. (*
   intro H.
   generalize dependent t'.
@@ -248,10 +510,10 @@ Proof. Admitted. (*
       rename X0 into IH_t_let_body.
       rename t0 into t_body.
 
-      assert (ex_dec_bs_true : { t_body & Bindings_desugar' Term_desugar bs t' = Just t_body}).
+      assert (ex_dec_bs_true : { t_body & dec_Bindings' dec_Term bs t' = Just t_body}).
         { destruct bs.
           { inversion H_dec_true. }
-          { destruct (Bindings_desugar' Term_desugar (b :: bs) t')
+          { destruct (dec_Bindings' dec_Term (b :: bs) t')
               eqn:dec_b_bs_true.
               2: { inversion H_dec_true. }
               eapply existT.
@@ -260,10 +522,10 @@ Proof. Admitted. (*
         }
       destruct ex_dec_bs_true as [ t_body' dec_bs_true ].
 
-      assert (dec_t_body_true : Term_desugar t_body t_body' = true).
+      assert (dec_t_body_true : dec_Term t_body t_body' = true).
         { destruct bs.
           { inversion H_dec_true. }
-          { destruct (Bindings_desugar' Term_desugar (b :: bs) t')
+          { destruct (dec_Bindings' dec_Term (b :: bs) t')
               eqn:dec_b_bs_true.
               2: { inversion H_dec_true. }
             inversion dec_bs_true.
@@ -414,14 +676,14 @@ Defined.*)
 
 
 Definition Binding_completeness (b : Binding) :=
-  forall s v t, b = TermBind s v t -> forall t', CNR_Term t t' -> Term_desugar t t' = true.
+  forall s v t, b = TermBind s v t -> forall t', CNR_Term t t' -> dec_Term t t' = true.
 
 Definition Term_completeness (t : Term) :=
-  forall t', CNR_Term t t' -> Term_desugar t t' = true .
+  forall t', CNR_Term t t' -> dec_Term t t' = true .
 
 
 
-Definition Term_desugar_complete t : forall t', CNR_Term t t' -> Term_desugar t t' = true .
+Definition dec_Term_complete t : forall t', CNR_Term t t' -> dec_Term t t' = true .
 Proof. Admitted.
 (*
 Proof.
