src/PlutusIR/Transform/LetNonRec/Spec.v
@@ -12,13 +12,34 @@ Import Coq.Lists.List.ListNotations.
    Desugaring strict, non-recursive lets into lambda-applications
 *)
 Inductive CNR_Term : Term -> Term -> Prop :=
-  | CNR_Let : forall {bs t_body t_body' f_bs},
+  | CNR_LetNonRec : forall {bs t_body t_body' f_bs},
       CNR_Term t_body t_body' ->
       CNR_Bindings bs f_bs ->
       CNR_Term (Let NonRec bs t_body) (fold_right apply t_body' f_bs )
+
+  (* Compatibility cases *)
+  | CNR_LetRec : forall bs bs' t_body t_body',
+      CNR_Term t_body t_body' ->
+      CNR_LetRec_compat bs bs' ->
+      CNR_Term (Let Rec bs t_body) (Let Rec bs' t_body')
+  | CNR_Var : compat_Var CNR_Term
+  | CNR_TyAbs : compat_TyAbs CNR_Term
+  | CNR_LamAbs : compat_LamAbs CNR_Term
+  | CNR_Apply : compat_Apply CNR_Term
+  | CNR_Constant : compat_Constant CNR_Term
+  | CNR_Builtin : compat_Builtin CNR_Term
+  | CNR_TyInst : compat_TyInst CNR_Term
+  | CNR_Error : compat_Error CNR_Term
+  | CNR_IWrap : compat_IWrap CNR_Term
+  | CNR_Unwrap : compat_Unwrap CNR_Term
+  | CNR_Constr : compat_Constr CNR_Term
+  | CNR_Case : compat_Case CNR_Term
+
+  (*
   | CNR_Compat : forall {t t'},
       Compat CNR_Term t t' ->
       CNR_Term t t'
+      *)
 
 (*
   `CNR_Bindings bs fs` states that each binding
@@ -46,6 +67,31 @@ with CNR_Binding : Binding -> (Term -> Term) -> Prop :=
       CNR_Binding
         (TermBind Strict (VarDecl v ty) t_bound)
         (fun t_bs => Apply (LamAbs v ty t_bs) t_bound')
+with CNR_LetRec_compat : list Binding -> list Binding -> Prop :=
+  | CNR_LetRec_nil :
+      CNR_LetRec_compat [] []
+  | CNR_LetRec_cons : forall b b' bs bs',
+      CNR_Binding_compat b b' ->
+      CNR_LetRec_compat bs bs' ->
+      CNR_LetRec_compat (b::bs) (b'::bs')
+with CNR_Binding_compat : Binding -> Binding -> Prop :=
+  | CNR_TermBind : compat_TermBind CNR_Term CNR_Binding_compat
+  | CNR_DatatypeBind : compat_DatatypeBind CNR_Binding_compat
+  | CNR_TypeBind : compat_TypeBind CNR_Binding_compat
   .
 
 
+Scheme CNR__ind := Minimality for CNR_Term Sort Prop
+  with CNR_Bindings__ind := Minimality for CNR_Bindings Sort Prop
+  with CNR_Binding__ind := Minimality for CNR_Binding Sort Prop
+  with CNR_LetRec_compat__ind := Minimality for CNR_LetRec_compat Sort Prop
+  with CNR_Binding_compat__ind := Minimality for CNR_Binding_compat Sort Prop
+.
+
+Combined Scheme CNR__multind from
+  CNR__ind,
+  CNR_Bindings__ind,
+  CNR_Binding__ind,
+  CNR_LetRec_compat__ind,
+  CNR_Binding_compat__ind
+.
