src/Examples/Timelock.v
@@ -285,15 +285,11 @@ Definition plc_3_4 :
   plc_3_dbe = plc_4_inlined.
 Proof. reflexivity. Qed.
 
-(* Compute Term_desugar plc_4_inlined plc_5_compileNonRecTerms. *)
-
-Definition plc_4_5_true : Term_desugar plc_4_inlined plc_5_compileNonRecTerms = true.
-Proof. reflexivity. Qed.
-
 Definition plc_4_5 :
   CNR_Term plc_4_inlined plc_5_compileNonRecTerms.
 Proof.
-  exact (Term_desugar_sound _ _ (plc_4_5_true)).
+  apply dec_Term_equiv.
+  reflexivity.
 Qed.
 
 (*
