src/PlutusIR/Transform/LetNonRec/Misc.v
@@ -1,0 +1,115 @@
+From PlutusCert Require Import PlutusIR.
+Import NamedTerm.
+From PlutusCert Require Import PlutusIR.Transform.Compat.
+From PlutusCert Require Import PlutusIR.Analysis.FreeVars.
+Require Import Coq.Strings.String.
+Require Import Coq.Lists.List.
+Require Import Coq.Program.Basics.
+Import Coq.Lists.List.ListNotations.
+
+From PlutusCert Require Import LetNonRec.Spec.
+
+(* Functional specification of the pass *)
+Fixpoint compile_term (t : Term) : Term := match t with
+  | Let NonRec bs t => fold_right apply t (map compile_NonRec_Binding bs)
+  | Let Rec bs t    => Let Rec (map compile_Rec_Binding bs) (compile_term t)
+
+  | TyAbs α k t     => TyAbs α k (compile_term t)
+  | LamAbs x τ t    => LamAbs x τ (compile_term t)
+  | Apply t1 t2     => Apply (compile_term t1) (compile_term t2)
+  | IWrap σ τ t     => IWrap σ τ (compile_term t)
+  | Unwrap t        => Unwrap (compile_term t)
+  | TyInst t τ      => TyInst (compile_term t) τ
+
+  | Var x           => Var x
+  | Constant c      => Constant c
+  | Builtin f       => Builtin f
+  | Error τ         => Error τ
+  | Constr i ts     => Constr i (map compile_term ts)
+  | Case t ts       => Case (compile_term t) (map compile_term ts)
+  end
+
+with compile_NonRec_Binding (b : Binding) : Term -> Term :=
+  match b with
+  | TermBind Strict (VarDecl v ty) t_bound => fun t_bs => Apply (LamAbs v ty t_bs) (compile_term t_bound)
+  | _ => id
+  end
+
+with compile_Rec_Binding (b : Binding) : Binding := match b with
+  | TermBind Strict vd t_bound => TermBind Strict vd (compile_term t_bound)
+  | b => b
+  end
+  .
+
+(* Constructors where equalities in indices are made
+   explicit *)
+Ltac eq_principle :=
+  intros;
+  subst;
+  constructor;
+  assumption.
+
+Definition C_TyAbs' : forall R (t t' : Term) (n n' : string) (k k' : Kind),
+              n = n' -> k = k'
+              -> R t t' -> Compat R (TyAbs n k t) (TyAbs n' k' t').
+Proof. eq_principle. Qed.
+
+Definition C_LamAbs' : forall R (t t' : Term) (n n' : string) (ty ty': Ty),
+                n = n' -> ty = ty' -> R t t' -> Compat R (LamAbs n ty t) (LamAbs n' ty' t').
+Proof. eq_principle. Qed.
+
+Definition C_Var' : forall R (n n' : string), (n = n') -> Compat R (Var n) (Var n').
+Proof. eq_principle. Qed.
+
+Definition C_Let' : forall R (bs bs' : list Binding) (t t' : Term) (r r' : Recursivity),
+             r = r' ->
+             Compat_Bindings R bs bs' ->
+             R t t' -> Compat R (Let r bs t) (Let r' bs' t').
+Proof. eq_principle. Qed.
+
+Definition C_Apply' : forall R (s s' t t' : Term),
+               R s s' -> R t t' -> Compat R (Apply s t) (Apply s' t').
+Proof. eq_principle. Qed.
+Definition C_Constant' : forall R (v v' : @some valueOf), v = v' -> Compat R (Constant v) (Constant v').
+Proof. eq_principle. Qed.
+Definition C_Builtin' : forall R (f f' : DefaultFun), f = f' -> Compat R (Builtin f) (Builtin f').
+Proof. eq_principle. Qed.
+Definition C_TyInst' : forall R (t t' : Term) (ty ty' : Ty),
+                ty = ty' -> R t t' -> Compat R (TyInst t ty) (TyInst t' ty').
+Proof. eq_principle. Qed.
+
+Definition C_Error' : forall R (ty ty' : Ty), ty = ty' -> Compat R (Error ty) (Error ty').
+Proof. eq_principle. Qed.
+
+Definition C_IWrap' : forall R (t t' : Term) (ty1 ty1' ty2 ty2' : Ty),
+               ty1 = ty1' -> ty2 = ty2' -> R t t' -> Compat R (IWrap ty1 ty2 t) (IWrap ty1' ty2' t').
+Proof. eq_principle. Qed.
+Definition C_Unwrap' : forall R (t t' : Term), R t t' -> Compat R (Unwrap t) (Unwrap t').
+Proof. eq_principle. Qed.
+
+Create HintDb eq_principles.
+#[global]
+Hint Resolve C_Let' C_Var' C_LamAbs' C_TyAbs' C_Apply' C_Constant' C_Builtin' C_TyInst' C_Error' C_IWrap' C_Unwrap : eq_principles.
+
+(*
+Definition CNR_Let' : forall (bs : list Binding) (t1 t1' t2 t2' t3 t3' : Term),
+  t1 = t1' -> t2 = t2' -> t3 = t3' ->
+  CNR_Term t1 t2 ->
+  CNR_Bindings bs f_bs -> CNR_Term (Let NonRec bs t1') t3'.
+Proof. intros. subst. eapply CNR_Let.
+  + apply X.
+  + apply X0.
+  Qed.
+*)
+
+Definition CNR_Desugar'
+    : forall v v' t_bound t_bound' ty,
+        v = v' ->
+        CNR_Term t_bound t_bound' ->
+        CNR_Binding
+          (TermBind Strict (VarDecl v ty) t_bound)
+          (fun t_bs => Apply (LamAbs v' ty t_bs) t_bound').
+Proof.
+  intros. subst. apply CNR_Desugar. assumption.
+Qed.
+
